Improve statement

pcuic/theories/PCUICSigmaCalculus.v
@@ -22,16 +22,52 @@ Open Scope sigma_scope.
 Definition well_subst Σ (Γ : context) σ (Δ : context) :=
   forall x decl,
     nth_error Γ x = Some decl ->
-    Σ ;;; Δ |- σ x : (decl_type decl).[ σ ].
+    Σ ;;; Δ |- σ x : ((lift0 (S x)) (decl_type decl)).[ σ ].
 
 Notation "Σ ;;; Δ ⊢ σ : Γ" :=
   (well_subst Σ Γ σ Δ) (at level 50, Δ, σ, Γ at next level).
 
+Lemma well_subst_Up :
+  forall Σ Γ Δ σ na A,
+    Σ ;;; Δ ⊢ σ : Γ ->
+    Σ ;;; Δ ,, vass na A.[σ] ⊢ ⇑ σ : Γ ,, vass na A.
+Proof.
+  intros Σ Γ Δ σ na A h [|n] decl e.
+  - simpl in *. inversion e. subst. clear e. simpl.
+    (* NEED commutation lemma between lift and inst *)
+    admit.
+  - simpl in *.
+    specialize (h _ _ e).
+Admitted.
+
 Lemma type_inst :
   forall Σ Γ Δ σ t A,
+    wf Σ.1 ->
+    wf_local Σ Γ ->
+    wf_local Σ Δ ->
     Σ ;;; Δ ⊢ σ : Γ ->
     Σ ;;; Γ |- t : A ->
     Σ ;;; Δ |- t.[σ] : A.[σ].
-Abort.
+Proof.
+  intros Σ Γ Δ σ t A hΣ hΓ hΔ hσ h.
+  revert Σ hΣ Γ hΓ t A h Δ σ hΔ hσ.
+  apply (typing_ind_env (fun Σ Γ t T => forall Δ σ,
+    wf_local Σ Δ ->
+    Σ ;;; Δ ⊢ σ : Γ ->
+    Σ ;;; Δ |- t.[σ] : T.[σ]
+  )).
+  - intros Σ wfΣ Γ wfΓ n decl e X Δ σ hΔ hσ. simpl.
+    eapply hσ. assumption.
+  - intros Σ wfΣ Γ wfΓ l X H0 Δ σ hΔ hσ. simpl.
+    econstructor. all: assumption.
+  - intros Σ wfΣ Γ wfΓ na A B s1 s2 X hA ihA hB ihB Δ σ hΔ hσ.
+    autorewrite with sigma. simpl.
+    econstructor.
+    + eapply ihA ; auto.
+    + eapply ihB.
+      * econstructor ; auto.
+        eexists. eapply ihA ; auto.
+      * eapply well_subst_Up. assumption.
+Admitted.
 
 End Sigma.
